x86/ArgPassing.v
@@ -1,0 +1,203 @@
+Require Import CoqlibC Maps.
+Require Import ValuesC.
+Require Import MemoryC Integers AST.
+Require Import LocationsC Stacklayout Conventions.
+(** newly added **)
+Require Import AsmregsC.
+Require Mach.
+
+Set Implicit Arguments.
+
+
+(* Notation rtc := (Relation_Operators.clos_refl_trans_1n _). (* reflexive transitive closure *) *)
+(* Definition stores: mem -> mem -> Prop := *)
+(*   rtc (fun m0 m1 => exists chunk ptr val, Mem.storev chunk m0 ptr val = Some m1). *)
+
+Local Opaque Z.mul Z.add Z.div Z.sub.
+Local Opaque list_nth_z.
+
+(* A: RTL: list val *)
+(* B: Linear/LTL: Mach.regset + slot (locset) *)
+(* C: Mach: Mach.regset + mem *)
+(* D: Asm: Asm.regset + mem *)
+
+Section STYLES.
+
+  Variable sg: signature.
+  About Mach.extcall_arguments.
+  Print Mach.extcall_arg.
+  About extcall_arguments.
+
+  Inductive A2B (vs: list val) (ls: locset): Prop :=
+  | A2B_intro
+      (ARGS: vs = (map (fun p => Locmap.getpair p ls) (loc_arguments sg)))
+      (BOUND: 4 * size_arguments sg <= Ptrofs.max_unsigned)
+  .
+
+  Inductive B2C (m0: mem) (ls: locset) (m1: mem) (mrs: Mach.regset) (rsp: val): Prop :=
+  | B2C_intro
+      (REGS: forall
+          mr
+        ,
+          ls (R mr) = mrs mr)
+      m_alloc blk
+      (ALLOC: Mem.alloc m0 fe_ofs_arg (4 * (size_arguments sg)) = (m_alloc, blk))
+      (NB: m_alloc.(Mem.nextblock) = m1.(Mem.nextblock))
+      (PERM: all4 (Mem.perm m_alloc <4> Mem.perm m1))
+      (SLOTS: forall
+          l0
+          (IN: In l0 (regs_of_rpairs (loc_arguments sg)))
+        ,
+          match l0 with
+          | S Outgoing ofs ty =>
+            Mach.load_stack m1 rsp ty (Ptrofs.repr (fe_ofs_arg + 4 * ofs)) = Some (ls l0)
+          | _ => True
+          end)
+      (UNCH: Mem.unchanged_on top2 m0 m1)
+      (RSPPTR: rsp = (Vptr blk Ptrofs.zero true))
+      (BOUND: 4 * size_arguments sg <= Ptrofs.max_unsigned)
+  .
+  (* Inductive B2C (m0: mem) (ls: locset) (m1: mem) (mrs: Mach.regset) (rsp: val): Prop := *)
+  (* | B2C_intro *)
+  (*     (REGS: forall *)
+  (*         mr *)
+  (*       , *)
+  (*         ls (R mr) = mrs mr) *)
+  (*     (NB: Pos.succ m0.(Mem.nextblock) = m1.(Mem.nextblock)) *)
+  (*     (RSPPTR: rsp = (Vptr m0.(Mem.nextblock) Ptrofs.zero true)) *)
+  (*     (PERM: Mem.range_perm m1 m0.(Mem.nextblock) 0 (4 * (size_arguments sg)) Cur Freeable) *)
+  (*     (SLOTS: forall *)
+  (*         l0 *)
+  (*         (IN: In l0 (regs_of_rpairs (loc_arguments sg))) *)
+  (*       , *)
+  (*         match l0 with *)
+  (*         | S Outgoing ofs ty => *)
+  (*           Mach.load_stack m1 rsp ty (Ptrofs.repr (fe_ofs_arg + 4 * ofs)) = Some (ls l0) *)
+  (*         | _ => True *)
+  (*         end) *)
+  (*     (UNCH: Mem.unchanged_on top2 m0 m1) *)
+  (*     (BOUND: 4 * size_arguments sg <= Ptrofs.max_unsigned) *)
+  (* . *)
+
+  Compute (to_mreg RSP).
+  Compute (to_mreg PC).
+  Compute (to_mreg RA).
+
+  Inductive C2D (mrs: Mach.regset) (fptr: val) (rsp: val) (prs: Asmregs.regset): Prop :=
+  | C2D_intro
+      ra
+      (REGSET: prs = fun pr =>
+                       match to_mreg pr with
+                       | Some mr => mrs mr
+                       | None =>
+                         match pr with
+                         | RSP => rsp
+                         | PC => fptr
+                         | RA => ra
+                         | _ => Vundef
+                         end
+                       end)
+      (RAPTR: is_ptr ra)
+  .
+
+  Inductive D2A (prs_arg: regset) (m_arg: mem)
+            (fptr_init: val) (vs_init: list val) (m_init: mem): Prop :=
+  | D2A_intro
+      sp
+      (RSPPTR: prs_arg RSP = Vptr sp Ptrofs.zero true)
+      (FPTR: prs_arg PC = fptr_init)
+      (PERM: Mem.range_perm m_arg sp 0 (4 * (size_arguments sg)) Cur Writable)
+      (VAL: extcall_arguments prs_arg m_arg sg vs_init)
+      (DROP: Mem_drop_perm_none m_arg sp 0 (4 * (size_arguments sg)) = m_init)
+      (RAPTR: is_ptr (prs_arg RA))
+      (BOUND: DUMMY_PROP) (* 4 * size_arguments sg <= Ptrofs.max_unsigned) *)
+  .
+
+  Inductive A2D (fptr_arg: val) (vs_arg: list val) (m_arg_pre: mem)
+             (prs_arg: Asmregs.regset) (m_arg: mem): Prop :=
+  | A2D_intro
+      ls
+      (AB: A2B vs_arg ls)
+      mrs rsp_arg
+      (BC: B2C m_arg_pre ls m_arg mrs rsp_arg)
+      (CD: C2D mrs fptr_arg rsp_arg prs_arg)
+  .
+
+  Lemma A2D_progress
+        fptr vs m0
+        (BOUND: 4 * size_arguments sg <= Ptrofs.max_unsigned)
+    :
+      exists prs m1, <<AD: A2D fptr vs m0 prs m1>>
+  .
+  Proof.
+    admit "This is needed for user to reason about their program. (or to prove refinement of C-phys >= C-logic)
+This is a complex job, and Compcert avoided it by translation validation.
+We might need to revert some old code.
+NOTE: Old version of Compcert should have related code.
+> 6224148 - (HEAD -> master) Reorganization test directory (2010-02-17 13:44:32 +0000) <xleroy>
+I checked this commit, there is a pass called Reload which deals this problem.".
+  Qed.
+
+  Lemma A2D2A
+        fptr vs m0 prs m1
+        (AD: A2D fptr vs m0 prs m1)
+    :
+      exists m2, <<DA :D2A prs m1 fptr vs m2>> /\ <<MEM: mem_equiv m0 m2>>
+  .
+  Proof.
+    inv AD.
+    inv AB; inv BC; inv CD. ss.
+    esplits; eauto.
+    - econs; cbn; eauto.
+      + ii. eapply PERM. eapply Mem.perm_implies; eauto with mem.
+      + hnf.
+        generalize (loc_arguments_acceptable_2 sg). intro ACCPS.
+        generalize (loc_arguments_one sg). intro ONES.
+        abstr (loc_arguments sg) locs.
+        clears sg; clear sg.
+        clear - ACCPS ONES SLOTS REGS.
+        ginduction locs; ii; ss.
+        * econs; eauto.
+        * econs; eauto; cycle 1.
+          { eapply IHlocs; eauto.
+            - ii. eapply SLOTS; eauto. apply in_app_iff. eauto.
+            - ii. eapply ACCPS. eauto. apply in_app_iff. eauto. }
+          exploit ONES; eauto. i; des.
+          destruct a; ss.
+          destruct r; ss; econs; eauto.
+          -- erewrite REGS. rpapply extcall_arg_reg. u. rewrite to_preg_to_mreg. ss.
+          -- exploit ACCPS; eauto. intro ACCP. ss. des_ifs.
+             econs; eauto. exploit SLOTS; eauto.
+    - hexploit (Mem_drop_perm_none_spec m1 m0.(Mem.nextblock) 0 (4 * size_arguments sg)); eauto. i; des.
+      exploit Mem.alloc_result; eauto. i; des. clarify.
+      econs; eauto.
+      + eapply Mem_unchanged_on_trans_strong; eauto.
+        eapply Mem.unchanged_on_implies; eauto.
+        ii; des.
+        left. ii. unfold Mem.valid_block in *. subst. xomega.
+      + i. rewrite <- NB0 in *. rewrite <- NB in *.
+        assert(b = Mem.nextblock m0).
+        { admit "ez". }
+        clarify.
+        eapply drop_perm_none_dead_block; eauto. ii; ss.
+        rewrite <- PERM in PERM0.
+        eapply Mem.perm_alloc_3; eauto.
+  Unshelve.
+    all: ss.
+  Qed.
+
+  Lemma mem_future
+    :
+      True
+  .
+  Proof.
+    admit "
+Two possibilities.
+1) all these operations can be presented with memory primitives. (alloc/store/etc)
+2) put these as primitive, and show that they comply to axioms. (readonly things)
+".
+  Qed.
+
+End STYLES.
+
+
